chapter {* camr project *}

theory Unification imports Main begin

(* Assignment 1 *)

(****************************** definitions ******************************)

datatype ('f, 'v) "term" = Var 'v | Fun 'f "('f, 'v) term list"

fun fv :: "('f, 'v) term \<Rightarrow> 'v set" where
  "fv (Var x) = {x}"
| "fv (Fun f xs) = (\<Union>x \<in> (set xs). fv x)"

type_synonym ('f, 'v) subst = "'v \<Rightarrow> ('f, 'v) term"

fun sapply :: "('f, 'v) subst \<Rightarrow> ('f, 'v) term \<Rightarrow> ('f, 'v) term" (infixr "\<cdot>" 67) where 
  "sapply \<sigma> (Var x) = \<sigma> x"
| "sapply \<sigma> (Fun g xs) = Fun g (map (sapply \<sigma>) xs)"

fun scomp :: "('f, 'v) subst \<Rightarrow> ('f, 'v) subst \<Rightarrow> ('f, 'v) subst" (infixl "\<circ>s" 75) where
  "scomp \<sigma> \<tau> = (\<lambda>x. \<sigma> \<cdot> (\<tau> x))"



(******************************** lemmata **********************************) 

lemma fv_sapply: "fv (\<sigma> \<cdot> t) = (\<Union>x \<in> fv t. fv (\<sigma> x))"
  apply (induction t rule: fv.induct)
   apply (auto)
  done

lemma sapply_cong: "\<lbrakk>\<And>x. x \<in> fv t \<Longrightarrow> \<sigma> x = \<tau> x \<rbrakk> \<Longrightarrow> \<sigma> \<cdot> t = \<tau> \<cdot> t"
  apply (induction t rule: fv.induct)
   apply (auto)
  done

lemma scomp_sapply [simp]: "(\<sigma> \<circ>s \<tau>) x = \<sigma> \<cdot> (\<tau> x)"
  by simp

lemma sapply_scomp_distr [simp]: "(\<sigma> \<circ>s \<tau>) \<cdot> t = \<sigma> \<cdot> (\<tau> \<cdot> t)"
  apply simp
  apply (induction t rule: fv.induct)
   apply auto
  done

lemma scomp_assoc: "(\<sigma> \<circ>s \<tau>) \<circ>s \<rho> = \<sigma> \<circ>s (\<tau> \<circ>s \<rho>)"
proof -
  have "(\<sigma> \<circ>s \<tau>) \<circ>s \<rho> = (\<lambda>x. (\<sigma> \<circ>s \<tau>) \<cdot> \<rho> x)" by simp
  also have "... = (\<lambda>x. \<sigma> \<cdot> \<tau> \<cdot> \<rho> x)" by (simp only: sapply_scomp_distr)
  also have "... = \<sigma> \<circ>s (\<tau> \<circ>s \<rho>)" by simp
  finally show ?thesis .
qed

lemma scomp_var [simp]: "\<sigma> \<circ>s Var = \<sigma>"
  by simp

lemma var_sapply: "Var \<cdot> t = t"
  apply (induction t rule: fv.induct)
  by (auto simp add: map_idI)

lemma var_scomp [simp]: "Var \<circ>s \<sigma> = \<sigma>"
  by (simp add: var_sapply)


(********************************** definitions ****************************)

fun sdom :: "('f, 'v) subst \<Rightarrow> 'v set" where
  "sdom \<sigma> = {x | x. \<sigma> x \<noteq> Var x}"

fun ran :: "('f, 'v) subst \<Rightarrow> ('f, 'v) term set" where
  "ran \<sigma> = {\<sigma> x | x. x \<in> sdom \<sigma>}"

fun svran :: "('f, 'v) subst \<Rightarrow> 'v set" where
  "svran \<sigma> = (\<Union> t \<in> ran \<sigma>. fv t)"


(************************************ lemmata ******************************)

lemma sdom_var [simp]: "sdom Var = {}"
  by simp

lemma svran_var [simp]: "svran Var = {}"
  by simp

lemma sdom_single_non_trivial [simp]: "t \<noteq> Var x \<Longrightarrow> sdom (Var (x := t)) = {x}"
  by simp

lemma svran_single_non_trivial [simp]: "t \<noteq> Var x \<Longrightarrow> svran (Var (x := t)) = fv t"
  by simp

(*lemma "\<sigma> \<cdot> t = (fv t - sdom \<sigma>) \<union> ran \<sigma>"*)


lemma fv_sapply_sdom_svran: "x \<in> fv (\<sigma> \<cdot> t) \<Longrightarrow> x \<in> (fv t - sdom \<sigma>) \<union> svran \<sigma>"
  apply (induction t rule: fv.induct)
  sorry


lemma sdom_scomp: "sdom (\<sigma> \<circ>s \<tau>) \<subseteq> sdom \<sigma> \<union> sdom \<tau>"
  sorry

lemma svran_scomp: "svran (\<sigma> \<circ>s \<tau>) \<subseteq> svran \<sigma> \<union> svran \<tau>"
  sorry


(**************************************** definitions *********************************)

type_synonym ('f, 'v) equation = "('f, 'v) term \<times> ('f, 'v) term"

type_synonym ('f, 'v) equations = "('f, 'v) equation list"

fun fv_eq :: "('f, 'v) equation \<Rightarrow> 'v set \<times> 'v set" where
  "fv_eq (a, b) = (fv a, fv b)"

fun fv_eqs :: "('f, 'v) equations \<Rightarrow> ('v set \<times> 'v set) list" where
  "fv_eqs l = map fv_eq l"

fun sapply_eq :: "('f, 'v) subst \<Rightarrow> ('f, 'v) equation \<Rightarrow> ('f, 'v) equation" where
  "sapply_eq \<sigma> (a,b) = (sapply \<sigma> a, sapply \<sigma> b)"

fun sapply_eqs :: "('f, 'v) subst \<Rightarrow> ('f, 'v) equations \<Rightarrow> ('f, 'v) equations" where
  "sapply_eqs \<sigma> l = map (sapply_eq \<sigma>) l"


(******************************** lemmata *************************************)

lemma fv_sapply_eq: "fv_eq (sapply_eq \<sigma> (a,b)) = ((\<Union>x \<in> fv a. fv (\<sigma> \<cdot> a)), (\<Union>y \<in> fv b. fv (\<sigma> \<cdot> b)))"
  sorry

lemma fv_sapply_eqs: "set (fv_eqs (sapply_eqs \<sigma> l)) = (\<Union>x \<in> set l. fv_eq (sapply_eq \<sigma> x))"

lemma sapply_scomp_distrib_eq

lemma sapply_scomp_distrib_eqs


  
  



end
